* Added a small new theory about fixed points (least, and greatest) and   monotone functions. * Added an export_rewrites clause to the end of pred_setScript.  (No more   having to write SIMP_TAC std_ss [IN_UNION, IN_DELETE, IN_SING,....]) * Added SET_SPEC_CONV to the stateful rewriter and also to the PRED_SET_ss   simpset fragment. * Added BIGINTER constant to pred_setTheory; companion to BIGUNION.

src/pred_set/src/pred_setLib.sig
@@ -11,4 +11,6 @@ sig
   val INSERT_CONV    : conv -> conv
   val IMAGE_CONV     : conv -> conv -> conv
 
+  val PRED_SET_ss    : simpLib.ssdata
+
 end;
