src/pred_set/src/pred_setLib.sml
@@ -1,12 +1,14 @@
 structure pred_setLib :> pred_setLib =
 struct
 
-  
+
 
   open Abbrev PFset_conv;
   local open pred_setTheory in end;
 
   val SET_SPEC_CONV  = PGspec.SET_SPEC_CONV pred_setTheory.GSPECIFICATION
   val SET_INDUCT_TAC = PSet_ind.SET_INDUCT_TAC pred_setTheory.FINITE_INDUCT
-    
+
+  val PRED_SET_ss = pred_setSimps.PRED_SET_ss
+
 end;
