src/pred_set/src/pred_setSimps.sig
@@ -1,5 +1,16 @@
 signature pred_setSimps =
 sig
+  val SET_SPEC_ss : simpLib.ssdata
   val PRED_SET_ss : simpLib.ssdata
   val PRED_SET_AC_ss : simpLib.ssdata
 end
+
+(*
+   [SET_SPEC_ss] contains just the conversion PGspec.SET_SPEC_CONV, which
+   converts terms of the form x IN { z | ... }.
+
+   [PRED_SET_ss] is a combination of the above with the rewrite theorems
+   from pred_setTheory.pred_set_rwts.
+
+   [PRED_SET_AC_ss] AC-normalises union and intersection terms.
+*)
